all functions completed

Homework6.dfy
@@ -19,7 +19,7 @@ decreases xs
 {
 	match xs
         case Nil => ys
-        case Cons(x,xs') => Cons(x, append(xs',ys))
+        case Cons(x,xs_1) => Cons(x, append(xs_1,ys))
 }
 
 function treeContains<T>(tree:Tree<T>, element:T):bool
@@ -28,22 +28,57 @@ decreases tree
 {
 	match tree
         case Leaf => false
-        case Node(left, right, t) => t == element || treeContains(left, element) || treeContains(right, element)
+        case Node(l, r, t) => t == element || treeContains(l, element) || treeContains(r, element)
 }
-
 
 function listContains<T>(xs:List<T>, element:T):bool
 ensures xs == Nil ==> listContains(xs, element) == false
 decreases xs
 {
 	match xs
-        case Nil => false
-        case Cons(x, xs') => x == element || listContains(xs', element)
+    case Nil => false
+    case Cons(x, xs_1) => (x == element) || listContains(xs_1, element)
 }
 
 
-lemma sameElements<T>(tree:Tree<T>, element:T)
-ensures treeContains(tree, element) <==> listContains(flatten(tree), element)
+
+lemma member_to_list<T>(x:T,ys:List<T>,zs:List<T>)
+decreases ys
+decreases zs
+ensures listContains(append(ys,zs), x) == (listContains(ys, x) || listContains(zs, x))
 {
-	
+    match ys
+    case Nil => {}
+    case Cons(y,ys_1) => {
+        member_to_list(x,ys_1,zs);
+        assert listContains(append(ys_1,zs),x) == (listContains(ys_1,x) || listContains(zs,x));
+        assert listContains(append(ys,zs),x)
+            == listContains(append(Cons(y,ys_1),zs),x)
+            == listContains(Cons(y,append(ys_1,zs)),x)
+            == (x==y || listContains((append(ys_1,zs)),x))
+            == (x==y || listContains(ys_1,x) || listContains(zs,x))
+            == (listContains(Cons(y,ys_1),x) || listContains(zs,x))
+            == (listContains(ys,x)          || listContains(zs,x))
+            ;
+    }
+}
+
+lemma sameElements<T>(tree:Tree<T>, element:T)
+decreases tree
+ensures treeContains(tree, element) <==> listContains(flatten(tree), element)
+{ 
+    match tree
+    case Leaf => {}
+    case Node(l, r, t) => {
+        sameElements(l, element);
+        sameElements(r, element);
+        member_to_list(element,flatten(l),flatten(r));
+        assert treeContains(Node(l, r, t), element)
+            == (treeContains(l, element) || treeContains(r, element) || t == element)
+            == (listContains(flatten(l), element) || listContains(flatten(r), element) || t == element)
+            == (listContains(append(flatten(l),flatten(r)), element) || t == element)
+            == listContains (Cons(t, append(flatten(l),flatten(r))), element)
+            == listContains(flatten(Node(l, r, t)), element)
+            ;
+    }
 }
